SSA/Projects/SLLVM/Dialect/Semantics/Memory.lean
@@ -23,10 +23,17 @@ inductive Block where
   /-- A live piece of memory (i.e., has been allocated and not yet freed). -/
   | live (b : LiveBlock)
 
-structure MemoryState where
-  mem : Std.HashMap BlockId Block
+structure AllocState where
   nextFreeBlock : Nat
   deriving Inhabited
+
+structure MemoryState where
+  mem : Std.HashMap BlockId Block
+  deriving Inhabited
+
+structure GlobalState where
+  alloc : AllocState
+  mem : MemoryState
 
 structure Pointer where
   id : BlockId
@@ -49,13 +56,35 @@ def Pointer.offsetInBits (p : Pointer) : Nat :=
 /-! ## Refinement -/
 section Refinement
 
+instance : Refinement AllocState where
+  IsRefinedBy s t := s = t
+
 instance : Refinement MemoryState where
   IsRefinedBy s t := ∀ (id : BlockId),
     s[id]? = t[id]?
+
+instance : Refinement GlobalState where
+  IsRefinedBy s t :=
+    s.alloc ⊑ t.alloc ∧ s.mem ⊑ t.mem
+
+
+
+section Lemmas
+
+@[simp_sllvm]
+theorem GlobalState.isRefinedBy_iff (s t : GlobalState) :
+    s ⊑ t ↔ s.alloc ⊑ t.alloc ∧ s.mem ⊑ t.mem := by
+  rfl
+
+@[simp_sllvm]
+theorem AllocState.isRefinedBy_rfl (s : AllocState) :
+    s ⊑ s := by
+  rfl
 
 @[simp_sllvm]
 theorem MemoryState.isRefinedBy_rfl (s : MemoryState) :
     s ⊑ s := by
   intro id; rfl
 
+end Lemmas
 end Refinement
